move not working test at the top

iodiv/TauIODiv.Test.fst
@@ -3,10 +3,6 @@ module TauIODiv.Test
 open FStar.List.Tot
 open FStar.List.Tot.Properties
 open FStar.Tactics // Also defines forall_intro so place before Classical
-open FStar.Classical
-open FStar.IndefiniteDescription
-open FStar.Calc
-open FStar.FunctionalExtensionality
 
 open Util
 open Stream
@@ -16,6 +12,75 @@ open TauIODiv
 open DivFree
 open DivFreeTauSpec
 open DivFreeTauDM
+
+
+
+let body (fd : file_descr) : IODiv unit (requires fun hist -> is_open fd hist) (ensures fun hist r -> terminates r /\ 
+  (exists s. ret_trace r == [ERead fd s])) =
+  let msg = read fd in
+  ()
+
+let _repeat_with_inv 
+  (#pre:trace -> Type0)
+  (#inv:(trace -> Type0){forall h lt. pre h /\ inv lt ==> pre (rev_acc lt h)})
+  (body : iodiv_dm unit (iprepost (fun hist -> pre hist) (fun hist r -> terminates r /\ inv (ret_trace r)))) :
+  iodiv_dm
+    unit
+    (iprepost
+      (fun hist -> pre hist)
+      (fun hist r -> diverges r /\ repeat_inv_post inv r)
+    )
+= _repeat_with_inv_aux pre inv (dm_bind body (fun _ -> dm_ret (Inl ())))
+
+#set-options "--print_implicits"
+
+let repeat_with_inv 
+  (#pre:trace -> Type0)
+  (#inv:trace -> Type0)
+  (#c1:squash (forall h lt. pre h /\ inv lt ==> pre (rev_acc lt h)))
+  (body : unit -> IODiv unit pre (ensures fun hist r -> terminates r /\ inv (ret_trace r))) :
+  IODiv
+    unit
+    (requires fun hist -> pre hist)
+    (ensures fun hist r -> diverges r /\ repeat_inv_post inv r)
+= IODIV?.reflect (_repeat_with_inv #pre #inv (reify (body ())))
+
+[@"opaque_to_smt"]
+let myinv (fd:file_descr) : trace -> Type0 = fun tr -> exists s. tr == [ERead fd s]
+
+[@"opaque_to_smt"]
+let mypre (fd:file_descr) : trace -> Type0 = fun h -> is_open fd h
+
+val yes : (fd:file_descr) -> squash (forall h lt. mypre fd h /\ myinv fd lt ==> mypre fd (rev_acc lt h))
+let yes fd = 
+  reveal_opaque (`%mypre) mypre;
+  reveal_opaque (`%myinv) myinv
+
+[@"opaque_to_smt"]
+let body' (fd :file_descr) () : IODiv unit (mypre fd) (ensures fun hist r -> terminates r /\ myinv fd (ret_trace r)) =
+  reveal_opaque (`%mypre) mypre;
+  reveal_opaque (`%myinv) myinv;
+  body fd
+
+let repeat_with_inv' (fd:file_descr) = repeat_with_inv #(mypre fd) #(myinv fd) #(yes fd)
+
+let repeat_loop_body (fd : file_descr) : IODiv unit (mypre fd) (ensures fun hist r -> diverges r /\ repeat_inv_post (myinv fd) r) =
+  let body'' : (unit
+            -> IODiv unit (mypre fd) (fun _ r -> terminates #unit r /\ myinv fd (ret_trace #unit r))) = body' fd in
+  admit (); // TODO: why is this failing???
+  repeat_with_inv' fd body''
+  
+
+
+
+
+
+
+
+
+
+
+
 
 // let open_file (s : string) : IODiv file_descr (requires fun hist -> True) (ensures fun hist r -> terminates r /\ ret_trace r == [ EOpenfile s (result r) ]) =
 //   act_call Openfile s
@@ -154,70 +219,6 @@ let repeat_test (s : string) : IODiv unit (requires fun hist -> True) (ensures f
   ) false
 
 
-
-let body (fd : file_descr) : IODiv unit (requires fun hist -> is_open fd hist) (ensures fun hist r -> terminates r /\ 
-  (exists s. ret_trace r == [ERead fd s])) =
-  let msg = read fd in
-  ()
-
-let _repeat_with_inv 
-  (#pre:trace -> Type0)
-  (#inv:(trace -> Type0){forall h lt. pre h /\ inv lt ==> pre (rev_acc lt h)})
-  (body : iodiv_dm unit (iprepost (fun hist -> pre hist) (fun hist r -> terminates r /\ inv (ret_trace r)))) :
-  iodiv_dm
-    unit
-    (iprepost
-      (fun hist -> pre hist)
-      (fun hist r -> diverges r /\ repeat_inv_post inv r)
-    )
-= _repeat_with_inv_aux pre inv (dm_bind body (fun _ -> dm_ret (Inl ())))
-
-[@"opaque_to_smt"]
-let repeat_with_inv 
-  (#pre:trace -> Type0)
-  (#inv:trace -> Type0)
-  (#c1:squash (forall h lt. pre h /\ inv lt ==> pre (rev_acc lt h)))
-  (body : unit -> IODiv unit pre (ensures fun hist r -> terminates r /\ inv (ret_trace r))) :
-  IODiv
-    unit
-    (requires fun hist -> pre hist)
-    (ensures fun hist r -> diverges r /\ repeat_inv_post inv r)
-= IODIV?.reflect (_repeat_with_inv #pre #inv (reify (body ())))
-
-[@"opaque_to_smt"]
-let myinv (fd:file_descr) : trace -> Type0 = fun tr -> exists s. tr == [ERead fd s]
-
-[@"opaque_to_smt"]
-let mypre (fd:file_descr) : trace -> Type0 = fun h -> is_open fd h
-
-assume val yes : (fd:file_descr) -> squash (forall h lt. mypre fd h /\ myinv fd lt ==> mypre fd (rev_acc lt h))
-
-[@"opaque_to_smt"]
-let body' (fd :file_descr) () : IODiv unit (mypre fd) (ensures fun hist r -> terminates r /\ myinv fd (ret_trace r)) =
-  reveal_opaque (`%mypre) mypre;
-  reveal_opaque (`%myinv) myinv;
-  body fd
-
-let repeat_loop_body (fd : file_descr) : IODiv unit (mypre fd) (ensures fun hist r -> diverges r /\ repeat_inv_post (myinv fd) r) 
-by (explode (); 
-  tadmit ();
-  tadmit ();
-  tadmit ();
-  tadmit ();
-  tadmit ();
-  tadmit ();
-  tadmit ();
-  tadmit ();
-  tadmit ();
-  tadmit ();
-  tadmit ();
-  tadmit ();
-  tadmit ();
-
-dump "H") =
-  repeat_with_inv #(mypre fd) #(myinv fd) #(yes fd) (body' fd)
-//  repeat  (fun tr -> (exists s. tr == [ERead fd s])) body fd 
-  
 
 
 let repeat_test_aux1 (fd : file_descr) : IODiv unit (requires fun hist -> is_open fd hist) (ensures fun hist r -> diverges r /\ repeat_inv_post (fun tr -> exists s. tr == [ERead fd s]) r)
